paxos/proof_agreement_invariants.dfy
@@ -1,0 +1,214 @@
+include "types.dfy"
+include "network.dfy"
+include "agents.dfy"
+include "synod.dfy"
+
+module Proof_Agreement_Invs {
+import opened Network
+import opened Agents
+import opened Types
+import opened Synod
+
+
+/* All correct processes decide the same value */
+predicate Agreement(c:Constants, ds:DistrSys) 
+    requires c.WF()
+    requires ds.WF(c)
+{
+    forall i1, i2 | 
+        && c.ValidLdrIdx(i1) && LeaderHasDecided(c, ds, i1) 
+        && c.ValidLdrIdx(i2) && LeaderHasDecided(c, ds, i2) 
+    :: TwoLeadersHaveSameV(c, ds, i1, i2)
+}
+
+/* Invariants for establishing Agreement */
+predicate Agreement_Inv(c:Constants, ds:DistrSys) 
+{
+    && c.WF()
+    && ds.WF(c)
+    && Agreement(c, ds)
+    && Trivialities(c, ds)
+    && LdrAcceptsSetCorrespondToAcceptMsg(c, ds)
+    && LdrPromisesSetCorrespondToPromiseMsg(c, ds)
+    && AccPromisedBallotLargerThanAccepted(c, ds)
+    && AcceptMsgImpliesAccepted(c, ds)
+    && PromisedImpliesNoMoreAccepts(c, ds)
+    && (forall i | c.ValidLdrIdx(i) && LeaderHasDecided(c, ds, i) 
+        :: Agreement_Inv_Decided(c, ds, i)
+    )
+}
+
+
+/* Things that are true if v is decided with ballot b. */
+predicate Agreement_Inv_Decided(c:Constants, ds:DistrSys, i:int) 
+    requires c.WF() && ds.WF(c)
+    requires c.ValidLdrIdx(i) && LeaderHasDecided(c, ds, i) 
+{
+    var b, v := ds.leaders[i].ballot, ds.leaders[i].val;
+    && LargerBallotPhase2LeadersV(c, ds, v, b)
+    && LargerBallotAcceptors(c, ds, v, b)
+    && LargerBallotPromiseMsgs(c, ds, v, b)
+    && LargerBallotProposeMsgs(c, ds, v, b)
+    && LargerBallotsPromiseQrms(c, ds, b)
+    && LeaderHasQuorumOfAccepts(c, ds, i)
+}
+
+
+predicate Trivialities(c:Constants, ds:DistrSys) 
+    requires c.WF() && ds.WF(c)
+{
+    && LdrBallotNotBottom(c, ds)
+    && AllPacketsValid(c, ds)
+}
+
+
+
+
+/* All l.accepts collected by l came from network */
+predicate LdrAcceptsSetCorrespondToAcceptMsg(c:Constants, ds:DistrSys) 
+    requires c.WF() && ds.WF(c)
+{
+    forall i | c.ValidLdrIdx(i) ::(
+        forall s | s in ds.leaders[i].accepts
+        :: Packet(s, Id(Ldr, i), Accept(ds.leaders[i].ballot)) in ds.network.sentPackets
+    )
+}
+
+/* All l.promises collected by l came from network */
+predicate LdrPromisesSetCorrespondToPromiseMsg(c:Constants, ds:DistrSys) 
+    requires c.WF() && ds.WF(c)
+{
+    forall i | c.ValidLdrIdx(i) ::(
+        forall p | p in ds.leaders[i].promises
+        :: p in ds.network.sentPackets
+    )
+}
+
+/* Acceptor promised ballot always at least as large as accepted ballot */
+predicate AccPromisedBallotLargerThanAccepted(c:Constants, ds:DistrSys) 
+    requires c.WF() && ds.WF(c)
+{
+    forall i | c.ValidAccIdx(i) 
+    :: BalLtEq(ds.acceptors[i].accepted.b, ds.acceptors[i].promised)
+}
+
+
+/* If a promised packet promised b', with previously accepted (v, b), then there can be no 
+* accept messages in network, from the same acceptor, with ballot x 
+* such that b < x < b' */
+predicate PromisedImpliesNoMoreAccepts(c:Constants, ds:DistrSys) 
+    requires c.WF() && ds.WF(c)
+{
+    forall prom_p | 
+        && prom_p in ds.network.sentPackets 
+        && prom_p.msg.Promise?
+    :: 
+    var promised_bal := prom_p.msg.bal;
+    var accepted_bal := prom_p.msg.vb.b;
+    AcceptMessageConstraint(c, ds, prom_p.src, promised_bal, accepted_bal)
+}
+
+predicate AcceptMessageConstraint(c:Constants, ds:DistrSys, src:Id, promised_bal:Ballot, accepted_bal:Ballot) 
+    requires c.WF() && ds.WF(c)
+{
+    forall acc_p | 
+        && acc_p in ds.network.sentPackets 
+        && acc_p.src == src
+        && acc_p.msg.Accept?
+    :: 
+        || BalLtEq(acc_p.msg.bal, accepted_bal)
+        || BalLtEq(promised_bal, acc_p.msg.bal)
+}
+
+/* If an Accept msg in network with src x, ballot b, then balval of acceptor x 
+* has has ballot >= b */
+predicate AcceptMsgImpliesAccepted(c:Constants, ds:DistrSys) 
+    requires c.WF() && ds.WF(c)
+{
+    forall p | 
+        && p in ds.network.sentPackets 
+        && p.msg.Accept?
+        && c.ValidAccIdx(p.src.idx) 
+    ::
+        BalLtEq(p.msg.bal, ds.acceptors[p.src.idx].accepted.b)
+}
+
+predicate LdrBallotNotBottom(c:Constants, ds:DistrSys) 
+    requires c.WF() && ds.WF(c)
+{
+    && (forall l | l in ds.leaders :: l.ballot != Bottom)
+}
+
+
+
+/* If v is decided with ballot b, then all phase 2 leaders with ballots
+* b' >= b must be of v */
+predicate LargerBallotPhase2LeadersV(c:Constants, ds:DistrSys, v:Value, b:Ballot) 
+    requires c.WF() && ds.WF(c)
+{
+    forall i' | 
+        && c.ValidLdrIdx(i') 
+        && BalLtEq(b, ds.leaders[i'].ballot) 
+        && LeaderInPhase2(c, ds, i') 
+    :: LeaderHasValueV(c, ds, i', v)
+}
+
+/* If v is decided with ballot b, then for any acceptor that accepted a ballot b'>=b, 
+* the accepted value is v */
+predicate LargerBallotAcceptors(c:Constants, ds:DistrSys, v:Value, b:Ballot) 
+    requires c.WF() && ds.WF(c)
+{
+    forall i' | c.ValidAccIdx(i') && BalLtEq(b, ds.acceptors[i'].accepted.b)
+    :: AcceptorHasValueV(c, ds, i', v)
+}
+
+
+/* If v is decided with ballot b, then for any Promise msgs with valbal ballot b'>=b, 
+* the valbal value is v */
+predicate LargerBallotPromiseMsgs(c:Constants, ds:DistrSys, v:Value, b:Ballot) 
+    requires c.WF() && ds.WF(c)
+{
+    forall p | p in ds.network.sentPackets && p.msg.Promise? && BalLtEq(b, p.msg.vb.b)
+    :: p.msg.vb.v == v
+}
+
+/* If v is decided with ballot b, then for any Propose msgs with ballot b'>=b, 
+* the value is v */
+predicate LargerBallotProposeMsgs(c:Constants, ds:DistrSys, v:Value, b:Ballot) 
+    requires c.WF() && ds.WF(c)
+{
+    forall p | p in ds.network.sentPackets && p.msg.Propose? && BalLtEq(b, p.msg.bal)
+    :: p.msg.val == v
+}
+
+/* If v is decided with ballot b, then all Promise quorums for ballots
+* b' >= b must come from an acceptor that accepted (v, b) */
+predicate LargerBallotsPromiseQrms(c:Constants, ds:DistrSys, b:Ballot) 
+    requires c.WF() && ds.WF(c)
+{
+    forall b' | BalLt(b, b') 
+    :: LargerBalQuorumHasSeenB(c, ds, b, b')
+}
+
+predicate LargerBalQuorumHasSeenB(c:Constants, ds:DistrSys, b:Ballot, b':Ballot) 
+    requires c.WF() && ds.WF(c)
+{
+    forall qrm:set<Packet> | QuorumOfPromiseMsgs(c, ds, qrm, b') 
+    :: QuorumHasSeenB(c, ds, qrm, b)
+}
+
+predicate QuorumHasSeenB(c:Constants, ds:DistrSys, qrm:set<Packet>, b:Ballot) 
+    requires c.WF() && ds.WF(c)
+    requires forall p | p in qrm :: p.msg.Promise?
+{
+    exists p :: p in qrm && BalLtEq(b, p.msg.vb.b)
+}
+
+predicate LeaderHasQuorumOfAccepts(c:Constants, ds:DistrSys, i:int) 
+    requires c.WF() && ds.WF(c)
+    requires c.ValidLdrIdx(i)
+{
+    |ds.leaders[i].accepts| == c.f + 1
+}
+
+}
