paxos/proof_helper.dfy
@@ -2,14 +2,53 @@ include "types.dfy"
 include "network.dfy"
 include "agents.dfy"
 include "synod.dfy"
+include "proof_agreement_invariants.dfy"
 
 module Proof_Helper {
 import opened Network
 import opened Agents
 import opened Types
 import opened Synod
+import opened Proof_Agreement_Invs
 
-lemma QuorumIntersection(c:Constants, ds:DistrSys, p1_qrm:set<Packet>, p1_bal:Ballot, p2_qrm:set<Packet>, p2_bal:Ballot)
+
+lemma Lemma_DecidedImpliesQuorumOfAccepts(c:Constants, ds:DistrSys, idx:int) 
+    requires c.WF() && ds.WF(c)
+    requires c.ValidLdrIdx(idx) && LeaderHasDecided(c, ds, idx);
+    requires LdrAcceptsSetCorrespondToAcceptMsg(c, ds)
+    requires LeaderHasQuorumOfAccepts(c, ds, idx)
+    ensures exists qrm :: QuorumOfAcceptMsgs(c, ds, qrm, ds.leaders[idx].ballot)
+{
+    var l, b := ds.leaders[idx], ds.leaders[idx].ballot;
+    var qrm:set<Packet> := {};
+    var accepts := l.accepts;
+    var sentPackets := ds.network.sentPackets;
+    var i := 0;
+    while i < c.f + 1 
+        decreases c.f+1 - i
+        invariant |accepts| == c.f+1 - i
+        invariant |qrm| == i
+        invariant UniqueSources(qrm)
+        invariant forall s | s in accepts :: 
+            (forall p | p in qrm :: p.src != s)
+        invariant forall s | s in accepts :: s in l.accepts
+        invariant forall p | p in qrm :: p.msg.Accept?
+        invariant forall p | p in qrm :: p.msg.bal == b
+        invariant forall p | p in qrm :: p in sentPackets;
+        invariant forall p | p in qrm :: p.dst == Id(Ldr, idx);
+    {
+        var s :| s in accepts;
+        var pkt := Packet(s, Id(Ldr, idx), Accept(b));
+        qrm := qrm + {pkt};
+        accepts := accepts - {s};
+        i := i + 1;
+    }
+    assert QuorumOfAcceptMsgs(c, ds, qrm, b);
+}
+
+
+
+lemma lemma_QuorumIntersection(c:Constants, ds:DistrSys, p1_qrm:set<Packet>, p1_bal:Ballot, p2_qrm:set<Packet>, p2_bal:Ballot)
     requires c.WF() && ds.WF(c)
     requires AllPacketsValid(c, ds)
     requires QuorumOfPromiseMsgs(c, ds, p1_qrm, p1_bal)
